\subsection{Laplace Transform}

\begin{topics}
	\begin{topic}{Definition}
		The Laplace transform takes a function $f(t)$ and produces a function $F(s)$.
		\begin{equation}
			\laplace{f(t)} = F(s) = \int_0^{\infty} e^{-st} f(t) dt
		\end{equation}
	\end{topic}

	\begin{topic}{Linearity}
		\begin{equation}
			\laplace{k_1 f(t) + k_2 g(t)} = k_1 \laplace{f(t)} + k_2 \laplace{g(t)}
		\end{equation}
	\end{topic}

	\begin{topic}{Examples}
		\begin{topics}
			\begin{topic}{$f(t) = 1$}
				\begin{equation}
					\laplace{1} = \frac{1}{s},
				\end{equation}
				where $s>0$.
			\end{topic}

			\begin{topic}{$f(t) = t^n$}
				\begin{equation}
					\laplace{t^n} = \frac{n!}{s^{n+1}},
				\end{equation}
				where $n \in \N$.
			\end{topic}

			\begin{topic}{$f(t) = e^{at}$}
				For $s > a$,
				\begin{equation}
					\laplace{e^{at}} = \frac{1}{s-a}.
				\end{equation}
				For $s \leq a$, $\laplace{e^{at}}$ diverges.
			\end{topic}

			\begin{topic}{$f(t) = \cos kt$}
				\begin{equation}
					\laplace{\cos kt} = \frac{s}{s^2 + k^2}
				\end{equation}
			\end{topic}

			\begin{topic}{$f(t) = \sin kt$}
				\begin{equation}
					\laplace{\sin kt} = \frac{k}{s^2 + k^2}
				\end{equation}
			\end{topic}
		\end{topics}
	\end{topic}
\end{topics}
